

# MATH 70095 - Applicable Maths

## Autumn 2025 - Unassessed Coursework

**Deadline: 9 October 2025, 09:00 (UK time)**

---

You should submit a PDF document containing your answers to these questions, via the Blackboard VLE, by the deadline stated above. Your submission may be a scanned copy of handwritten answers, or a typed document; all submissions should be clear and legible, and should also ***show all of your working***. This coursework should involve approximately **3 hours** of effort.

Your submission will be marked and you will be provided with written feedback. The marks available for each question are indicated in square brackets. This mark ***will not*** count towards your overall grade for Applicable Maths.

**Plagiarism:** Your submission should be *your own work*. Note that software tools are used for plagiarism detection.

---

Q1) The following derivations are incorrect. For each one, clearly describe any errors that have been made, and give the correct answer. [5]

a)

$$f(x) = \frac{x}{x + e^{-x}} \implies f'(x) = \frac{(1 - e^{-x})x - (x + e^{-x})}{(x + e^{-x})^2} = \frac{-e^{-x}(x + 1)}{(x + e^{-x})^2}.$$

b)

$$\begin{aligned} \int_0^{\pi/4} x^2 \sin 2x \, dx &= \left[ 2x \cdot \left( -\frac{1}{2} \cos 2x \right) \right]_0^{\pi/4} + \int_0^{\pi/4} x \cos 2x \, dx \\ &= \left[ -x \cos 2x \right]_0^{\pi/4} + \left[ x \cdot \left( \frac{1}{2} \sin 2x \right) \right]_0^{\pi/4} + \frac{1}{2} \int_0^{\pi/4} \sin 2x \, dx \\ &= \frac{\pi}{8} + \frac{1}{4}. \end{aligned}$$

Q2) Consider the multivariate function  $f(x, y, z) = \log g(x, y) + \log h(y, z)$ , where  $x, y, z \in \mathbb{R}$  and  $g, h$  are both positive-valued bivariate functions. [9]

a) Derive a vector-valued expression for the gradient,  $\nabla f(x, y, z)$ .

b) Derive the Hessian matrix,  $H_f = \nabla^2 f(x, y, z)$ .

You should provide your answers in terms of the functions  $g$  and  $h$  and their derivatives.

Q3) Consider the 4-dimensional Euclidean vector space  $E = (\mathbb{R}^4, +, \cdot)$ , equipped with the usual Euclidean inner product  $\langle \cdot, \cdot \rangle$ . [6]

- a) Let  $U \subseteq \mathbb{R}^4$  be a subspace spanned by the vectors

$$\begin{bmatrix} 1 \\ 0 \\ 2 \\ 1 \end{bmatrix}, \begin{bmatrix} 2 \\ 1 \\ 1 \\ 0 \end{bmatrix} \text{ and } \begin{bmatrix} 0 \\ 2 \\ 1 \\ 3 \end{bmatrix}.$$

Using a projection matrix  $P$ , calculate the orthogonal projection of  $\underline{v} = [1, 2, 1, 3]^T$  onto  $U$ .

- b) Using the Gram matrix, show that the following vectors are linearly independent:

$$\begin{bmatrix} 1 \\ 0 \\ 2 \\ 1 \end{bmatrix}, \begin{bmatrix} 2 \\ 1 \\ 1 \\ 0 \end{bmatrix}, \begin{bmatrix} 0 \\ 2 \\ 1 \\ 3 \end{bmatrix} \text{ and } \begin{bmatrix} 2 \\ 1 \\ 1 \\ 2 \end{bmatrix}.$$

Q1) The following derivations are incorrect. For each one, clearly describe any errors that have been made, and give the correct answer. [5]

a)

$$f(x) = \frac{x}{x + e^{-x}} \implies f'(x) = \frac{(1 - e^{-x})x - (x + e^{-x})}{(x + e^{-x})^2} = \frac{-e^{-x}(x + 1)}{(x + e^{-x})^2}.$$

quotient rule: for  $f(x) = \frac{h(x)}{g(x)}$

$$f'(x) = \frac{h'(x)g(x) - h(x)g'(x)}{(g(x))^2}$$

$$f(x) = \frac{x}{x + e^{-x}} \implies \begin{array}{ll} h(x) = x & h'(x) = 1 \\ g(x) = x + e^{-x} & g'(x) = 1 - e^{-x} \end{array}$$

$$f'(x) = \frac{1(x + e^{-x}) - x(1 - e^{-x})}{(x + e^{-x})^2} = \frac{(x + e^{-x}) - (x - xe^{-x})}{(x + e^{-x})^2}$$

$$= \frac{e^{-x} + xe^{-x}}{(x + e^{-x})^2}$$

$$= \frac{e^{-x}(x + 1)}{(x + e^{-x})^2}$$

$$f'(x) = \frac{(1 - e^{-x})x - (x + e^{-x})}{(x + e^{-x})^2}$$

The question applies the quotient rule incorrectly, the (incorrect) rule used is:

$$f'(x) = \frac{h(x)g'(x) - h'(x)g(x)}{(g(x))^2} \quad \text{for } f(x) = \frac{h(x)}{g(x)}$$

as a result, the simplified answer ends up being negative, due to the mistake.

b)

$$\begin{aligned}
 \int_0^{\pi/4} x^2 \sin 2x \, dx &= \left[ \overset{\text{Incorrect term in by parts, should be } x^2}{2x} \left( -\frac{1}{2} \cos 2x \right) \right]_0^{\pi/4} + \int_0^{\pi/4} x \cos 2x \, dx \\
 &\overset{\text{Incorrect from by parts formula}}{=} \left[ \overset{\text{negation missed on by parts formula}}{-x} \cos 2x \right]_0^{\pi/4} + \left[ x \cdot \left( \frac{1}{2} \sin 2x \right) \right]_0^{\pi/4} \overset{\text{negation missed on by parts formula}}{+} \frac{1}{2} \int_0^{\pi/4} \sin 2x \, dx \\
 &= \frac{\pi}{8} \overset{\text{missed negative in by parts on previous line, should be } \frac{\pi}{8} - \frac{1}{4}}{+} \frac{1}{4}.
 \end{aligned}$$

Integration by parts:

$$\int u \, dv = uv - \int v \, du$$

$$u = x^2 \rightarrow du = 2x$$

$$dv = \sin 2x \rightarrow v = -\frac{1}{2} \cos 2x$$

$$\begin{aligned}
 \int_0^{\pi/4} x^2 \sin 2x \, dx &= \left[ x^2 \cdot -\frac{1}{2} \cos(2x) \right]_0^{\pi/4} - \int_0^{\pi/4} -\frac{1}{2} \cos 2x \cdot 2x \, dx \\
 &= \left[ -\frac{x^2}{2} \cos 2x \right]_0^{\pi/4} + \int_0^{\pi/4} x \cos 2x \, dx \\
 &= \left[ -\frac{x^2}{2} \cos 2x \right]_0^{\pi/4} + \left[ \frac{x}{2} \sin 2x \right]_0^{\pi/4} - \int_0^{\pi/4} \frac{1}{2} \sin 2x \, dx \\
 &= \left[ -\frac{x^2}{2} \cos 2x \right]_0^{\pi/4} + \left[ \frac{x}{2} \sin 2x \right]_0^{\pi/4} + \left[ \frac{1}{4} \cos 2x \right]_0^{\pi/4} \\
 &= \left[ \downarrow \right] \left[ 0 \cdot 0 \right] + \left[ \downarrow \right] \left[ \frac{\pi}{8} - 0 \right] + \left[ \downarrow \right] \left[ 0 - \frac{1}{4} \right] \\
 &= \frac{\pi}{8} - \frac{1}{4}
 \end{aligned}$$

Q2) Consider the multivariate function  $f(x, y, z) = \log g(x, y) + \log h(y, z)$ , where  $x, y, z \in \mathbb{R}$  and  $g, h$  are both positive-valued bivariate functions. [9]

- Derive a vector-valued expression for the gradient,  $\nabla f(x, y, z)$ .
- Derive the Hessian matrix,  $H_f = \nabla^2 f(x, y, z)$ .

You should provide your answers in terms of the functions  $g$  and  $h$  and their derivatives.

a) Recall gradient  $\nabla f(x, y, z) =$

$$\left[ \frac{df}{dx}, \frac{df}{dy}, \frac{df}{dz} \right]^T$$

$$f(x, y, z) = \log g(x, y) + \log h(y, z)$$

$$\frac{df}{dx} = \frac{1}{g(x, y)} \cdot \frac{dg}{dx}(x, y)$$

$$\frac{df}{dy} = \frac{1}{g(x, y)} \cdot \frac{dg}{dy}(x, y) + \frac{1}{h(y, z)} \cdot \frac{dh}{dy}(y, z)$$

$$\frac{df}{dz} = \frac{1}{h(y, z)} \cdot \frac{dh}{dz}(y, z)$$

$$\text{So } \nabla f(x, y, z) = \left[ \frac{df}{dx}, \frac{df}{dy}, \frac{df}{dz} \right]^T =$$

$$\begin{bmatrix} \frac{df}{dx} \\ \frac{df}{dy} \\ \frac{df}{dz} \end{bmatrix} = \begin{bmatrix} \frac{1}{g(x, y)} \cdot \frac{dg}{dx}(x, y) \\ \frac{1}{g(x, y)} \cdot \frac{dg}{dy}(x, y) + \frac{1}{h(y, z)} \cdot \frac{dh}{dy}(y, z) \\ \frac{1}{h(y, z)} \cdot \frac{dh}{dz}(y, z) \end{bmatrix}$$

b) Recall Hessian matrix is a matrix of all second order partial derivatives, i.e.:

$$H^2 = \begin{bmatrix} \frac{d^2 f}{dx_1^2} & \frac{d^2 f}{dx_1 dx_2} & \dots & \frac{d^2 f}{dx_1 dx_n} \\ \frac{d^2 f}{dx_2 dx_1} & \frac{d^2 f}{dx_2^2} & \dots & \frac{d^2 f}{dx_2 dx_n} \\ \vdots & \vdots & \ddots & \vdots \\ \frac{d^2 f}{dx_n dx_1} & \frac{d^2 f}{dx_n dx_2} & \dots & \frac{d^2 f}{dx_n^2} \end{bmatrix}$$

so  $\nabla^2 f(x, y, z) =$

$$\begin{bmatrix} \frac{d^2 f}{dx^2} & \frac{d^2 f}{dx dy} & \frac{d^2 f}{dx dz} \\ \frac{d^2 f}{dy dx} & \frac{d^2 f}{dy^2} & \frac{d^2 f}{dy dz} \\ \frac{d^2 f}{dz dx} & \frac{d^2 f}{dz dy} & \frac{d^2 f}{dz^2} \end{bmatrix}$$

define shorthand  $g = g(x, y)$   
 $h = h(y, z)$

$$g_x = \frac{dg}{dx} g_{xx} = \frac{dg}{dx^2} \text{ etc}$$

$$\frac{df}{dx} = \frac{1}{g(x, y)} \cdot \frac{dg}{dx}(x, y) = \frac{g_x}{g}$$

$$\frac{df}{dy} = \frac{1}{g(x, y)} \cdot \frac{dg}{dy}(x, y) + \frac{1}{h(y, z)} \cdot \frac{dh}{dy}(y, z) = \frac{g_y}{g} + \frac{h_y}{h}$$

$$\frac{df}{dz} = \frac{1}{h(y, z)} \cdot \frac{dh}{dz}(y, z) = \frac{h_z}{h}$$

$$\frac{d^2 f}{dx^2} = \frac{d}{dx} \left[ \frac{g_x}{g} \right] = \frac{g \cdot g_{xx} - g_x^2}{g^2} \quad (\text{quotient rule})$$

$$\frac{d^2 f}{dx dy} = \frac{d}{dy} \left[ \frac{df}{dx} \right] = \frac{d}{dy} \left[ \frac{g_x}{g} \right] = \frac{g \cdot g_{xy} - g_x \cdot g_y}{g^2}$$

$$\frac{d^2 f}{dx dz} = \frac{d}{dz} \left[ \frac{df}{dx} \right] = \frac{d}{dz} \left[ \frac{g_x}{g} \right] = 0$$

$$\frac{d^2 f}{dy^2} = \frac{d}{dy} \left[ \frac{df}{dy} \right] = \frac{d}{dy} \left[ \frac{g_y}{g} + \frac{h_y}{h} \right] = \frac{g \cdot g_{yy} - g_y^2}{g^2} + \frac{h \cdot h_{yy} - h_y^2}{h^2}$$

$$\frac{d^2 f}{dz dy} = \frac{d}{dz} \left[ \frac{df}{dy} \right] = \frac{d}{dz} \left[ \frac{g_y}{g} + \frac{h_y}{h} \right] = \frac{d}{dz} \left[ \frac{h_y}{h} \right] = \frac{h \cdot h_{yz} - h_y h_z}{h^2}$$

$$\frac{d^2 f}{dz^2} = \frac{d}{dz} \left[ \frac{df}{dz} \right] = \frac{d}{dz} \left[ \frac{h_z}{h} \right] = \frac{h \cdot h_{zz} - h_z^2}{h^2}$$

so

$$\nabla^2 f(x, y, z) =$$

$$\begin{bmatrix} \frac{g g_{xx} - g_x^2}{g^2} & \frac{g g_{xy} - g_x g_y}{g^2} & 0 \\ \frac{g g_{xy} - g_x g_y}{g^2} & \frac{g g_{yy} - g_y^2}{g^2} + \frac{h h_{yy} - h_y^2}{h^2} & \frac{h h_{yz} - h_y h_z}{h^2} \\ 0 & \frac{h h_{yz} - h_y h_z}{h^2} & \frac{h h_{zz} - h_z^2}{h^2} \end{bmatrix}$$

Q3) Consider the 4-dimensional Euclidean vector space  $E = (\mathbb{R}^4, +, \cdot)$ , equipped with the usual Euclidean inner product  $\langle \cdot, \cdot \rangle$ . [6]

a) Let  $U \subseteq \mathbb{R}^4$  be a subspace spanned by the vectors

$$\begin{bmatrix} 1 \\ 0 \\ 2 \\ 1 \end{bmatrix}, \begin{bmatrix} 2 \\ 1 \\ 1 \\ 0 \end{bmatrix} \text{ and } \begin{bmatrix} 0 \\ 2 \\ 1 \\ 3 \end{bmatrix}.$$

Using a projection matrix  $P$ , calculate the orthogonal projection of  $\underline{v} = [1, 2, 1, 3]^T$  onto  $U$ .

b) Using the Gram matrix, show that the following vectors are linearly independent:

$$\begin{bmatrix} 1 \\ 0 \\ 2 \\ 1 \end{bmatrix}, \begin{bmatrix} 2 \\ 1 \\ 1 \\ 0 \end{bmatrix}, \begin{bmatrix} 0 \\ 2 \\ 1 \\ 3 \end{bmatrix} \text{ and } \begin{bmatrix} 2 \\ 1 \\ 1 \\ 2 \end{bmatrix}.$$

$$\text{proj}_U(\underline{v}) = P\underline{v} = A(A^T A)^{-1} A^T \underline{v}$$

$$A = \begin{bmatrix} 1 & 2 & 0 \\ 0 & 1 & 2 \\ 2 & 1 & 1 \\ 1 & 0 & 3 \end{bmatrix}$$

$$A^T A = \begin{bmatrix} 1 & 0 & 2 & 1 \\ 2 & 1 & 1 & 0 \\ 0 & 2 & 1 & 3 \end{bmatrix} \begin{bmatrix} 1 & 2 & 0 \\ 0 & 1 & 2 \\ 2 & 1 & 1 \\ 1 & 0 & 3 \end{bmatrix} = \begin{bmatrix} 6 & 4 & 7 \\ 4 & 6 & 3 \\ 7 & 3 & 14 \end{bmatrix}$$

$$(A^T A)^{-1} = \begin{bmatrix} \frac{29}{126} & -\frac{23}{126} & -\frac{5}{126} \\ -\frac{23}{126} & \frac{37}{126} & -\frac{1}{126} \\ -\frac{5}{126} & -\frac{1}{126} & \frac{11}{126} \end{bmatrix} \text{ via calculator.}$$

$$A(A^T A)^{-1} A^T \underline{v} =$$

$$A(A^T A)^{-1} \begin{bmatrix} 1 & 0 & 2 & 1 \\ 2 & 1 & 1 & 0 \\ 0 & 2 & 1 & 3 \end{bmatrix} \begin{bmatrix} 1 \\ 2 \\ 1 \\ 3 \end{bmatrix} =$$



$$= A(A^T A^{-1}) \begin{bmatrix} 6 \\ 5 \\ 4 \end{bmatrix}$$

$$= A \begin{bmatrix} \frac{29}{126} & -\frac{23}{126} & -\frac{5}{126} \\ -\frac{23}{126} & \frac{37}{126} & -\frac{1}{126} \\ -\frac{5}{126} & -\frac{1}{126} & \frac{11}{126} \end{bmatrix} \begin{bmatrix} 6 \\ 5 \\ 4 \end{bmatrix}$$

$$= A \begin{bmatrix} 1 \\ 1 \\ 2 \end{bmatrix} = \begin{bmatrix} 1 & 2 & 0 \\ 0 & 1 & 2 \\ 2 & 1 & 3 \end{bmatrix} \begin{bmatrix} 1 \\ 1 \\ 2 \end{bmatrix} = \begin{bmatrix} 3 \\ 5 \\ 7 \end{bmatrix}$$

$$\text{Proj}_U(v) = \begin{bmatrix} 3 \\ 5 \\ 5 \\ 7 \end{bmatrix}$$

b) Gram matrix  $G = (\langle x_i, x_j \rangle)_{i,j=1}^4$

$$v_1 = \begin{bmatrix} 1 \\ 0 \\ 2 \\ 1 \end{bmatrix} \quad v_2 = \begin{bmatrix} 2 \\ 1 \\ 1 \\ 0 \end{bmatrix} \quad v_3 = \begin{bmatrix} 0 \\ 2 \\ 1 \\ 3 \end{bmatrix} \quad v_4 = \begin{bmatrix} 2 \\ 1 \\ 1 \\ 3 \end{bmatrix}$$

$$G = \begin{bmatrix} 6 & 4 & 5 & 6 \\ 4 & 6 & 3 & 6 \\ 5 & 3 & 14 & 9 \\ 6 & 6 & 9 & 10 \end{bmatrix}$$

$v_1, v_2, v_3, v_4$  independent  $\Leftrightarrow G$  is nonsingular  $\Leftrightarrow \det G \neq 0$

Recall modulo- $p$  invertibility trick

if  $\det(A) \not\equiv 0 \pmod{p} \Rightarrow \det(A) \neq 0$  over  $\mathbb{Z}$  or  $\mathbb{R}$   
and  $\det G \pmod{p} = \det(G \pmod{p})$

$$G \bmod 2 = \begin{bmatrix} 0 & 1 & 0 & 1 \\ 1 & 1 & 0 & 1 \\ 0 & 0 & 1 & 0 \\ 1 & 1 & 0 & 1 \end{bmatrix}$$

after row reduction, this will have  $\det = 0$ , so try with mod 3

$$G \bmod 3 = \begin{bmatrix} 0 & 1 & 2 & 0 \\ 1 & 0 & 0 & 0 \\ 2 & 0 & 2 & 0 \\ 0 & 0 & 0 & 1 \end{bmatrix}$$

Gaussian elimination

$$\Rightarrow \begin{bmatrix} 1 & 0 & 0 & 0 \\ 0 & 1 & 2 & 0 \\ 2 & 0 & 2 & 0 \\ 0 & 0 & 0 & 1 \end{bmatrix} \quad R_1 \leftrightarrow R_2 \quad (\text{Row swap multiplies det by } -1 \equiv 2 \bmod 3)$$

$$\Rightarrow \begin{bmatrix} 1 & 0 & 0 & 0 \\ 0 & 1 & 2 & 0 \\ 0 & 0 & 2 & 0 \\ 0 & 0 & 0 & 1 \end{bmatrix} \quad R_3 - 2R_1 \quad (\text{Does not affect det})$$

swap factor  $-1 \equiv 2 \bmod 3$

$$\text{upper singular, so } \det(G \bmod 3) \equiv (1 \cdot 1 \cdot 2 \cdot 1) \cdot 2 \equiv 2 \cdot 2 \equiv 4 \equiv 1 \bmod 3$$

$$\text{so } \det(G \bmod 3) \equiv 1 \bmod 3 \Rightarrow \det G \equiv 1 \bmod 3.$$

$\therefore$  As  $\det G \not\equiv 0 \bmod 3$ ,  $G$  is nonsingular over  $\mathbb{Z} \nsubseteq \mathbb{R}$ , so the vectors are linearly independent.